Prove bisim sound for coinductive trace equivalence.

Equiv/TraceEquiv.v
@@ -185,6 +185,165 @@ Proof.
     + eapply producesNondetPrefix; eauto.
 Qed.
 
+CoInductive diverges S `{StateType S} : S -> Prop :=
+| DivergesI σ σ'
+  : step σ EvtTau σ'
+    -> diverges σ'
+    -> diverges σ.
+
+CoInductive diverges_gen S `{StateType S} (r:S -> Prop) : S -> Prop :=
+| DivergesGenI σ σ'
+  : step σ EvtTau σ'
+    -> r σ'
+    -> diverges_gen r σ.
+
+Hint Constructors diverges_gen.
+
+Definition diverges' S `{StateType S} : S -> Prop :=
+  paco1 (@diverges_gen S _) bot1.
+
+Hint Unfold diverges'.
+
+Lemma diverges_gen_mon S `{StateType S}
+: monotone1 (@diverges_gen S _).
+Proof.
+  hnf; intros. inv IN.
+  - econstructor 1; eauto.
+Qed.
+
+Hint Resolve diverges_gen_mon : paco.
+
+Lemma diverges_diverges' S `{StateType S} (σ:S)
+: diverges σ -> diverges' σ.
+Proof.
+  revert σ. pcofix CIH.
+  intros. pfold.
+  inv H1.
+  econstructor; eauto.
+Qed.
+
+Lemma diverges'_diverges S `{StateType S} (σ:S)
+  : diverges' σ -> diverges σ.
+Proof.
+  revert σ.
+  cofix COH; intros.
+  assert (diverges_gen (paco1 (diverges_gen (S:=S)) bot1 \1/ bot1) σ).
+  punfold H0.
+  inv H1.
+  econstructor; eauto.
+  destruct H3; eauto. inv H3.
+Qed.
+
+Lemma diverges_reduction_closed S `{StateType S} (σ σ':S)
+: diverges σ -> star2 step σ nil σ'  -> diverges σ'.
+Proof.
+  intros. general induction H1; eauto using diverges.
+  destruct yl, y; simpl in *; try congruence.
+  inv H2.
+  exploit step_internally_deterministic.
+  eapply H. eapply H3. dcr; subst.
+  eapply IHstar2; eauto.
+Qed.
+
+Lemma diverges_never_activated S `{StateType S} (σ:S)
+: activated σ -> diverges σ -> False.
+Proof.
+  intros. inv H0. inv H1. dcr.
+  exploit step_internally_deterministic.
+  eapply H3. eapply H5. dcr; congruence.
+Qed.
+
+Lemma diverges_never_terminates S `{StateType S} (σ:S)
+: normal2 step σ -> diverges σ -> False.
+Proof.
+  intros. inv H1. eapply H0. firstorder.
+Qed.
+
+Lemma bisim_sound_diverges S `{StateType S} S' `{StateType S'} (σ:S) (σ':S')
+: bisim σ σ' -> diverges σ -> diverges σ'.
+Proof.
+  revert σ σ'. cofix COH; intros.
+  inv H1.
+  - eapply plus2_destr_nil in H4. dcr.
+    econstructor. eauto.
+    eapply COH; eauto.
+    eapply bisim'_bisim.
+    eapply bisim'_reduction_closed.
+    eapply bisim_bisim'. eapply H1. econstructor.
+    eapply (S_star2 EvtTau); eauto. econstructor.
+  - eapply diverges_reduction_closed in H3.
+    + exfalso. eapply (diverges_never_activated H5); eauto.
+    + eapply H2.
+  - eapply diverges_reduction_closed in H4.
+    + exfalso. eapply (diverges_never_terminates H6); eauto.
+    + eapply H2.
+Qed.
+
+CoInductive stream (A : Type) : Type :=
+| sil : stream A
+| sons : A -> stream A -> stream A.
+
+Arguments sil [A].
+
+CoInductive coproduces {S} `{StateType S} : S -> stream extevent -> Prop :=
+| CoProducesExtern (σ σ' σ'':S) evt L :
+    star2 step σ nil σ'
+      -> activated σ'
+      -> step σ' evt σ''
+      -> coproduces σ' L
+      -> coproduces σ (sons (EEvt evt) L)
+| CoProducesSilent (σ:S) :
+    diverges σ
+    -> coproduces σ sil
+| CoProducesTerm (σ:S) (σ':S) r
+  : result σ' = r
+    -> star2 step σ nil σ'
+    -> normal2 step σ'
+    -> coproduces σ (sons (EvtTerminate r) sil).
+
+Lemma coproduces_reduction_closed_step S `{StateType S} (σ σ':S) L
+: coproduces σ L -> step σ EvtTau σ'  -> coproduces σ' L.
+Proof.
+  intros. inv H0.
+  - exploit activated_star_reach. eapply H3. eauto.
+    eapply (S_star2 EvtTau); eauto. econstructor.
+    econstructor. eapply X. eauto. eauto. eauto.
+  - econstructor. eapply diverges_reduction_closed; eauto.
+    eapply (S_star2 EvtTau); eauto. econstructor.
+  - exploit star2_reach_normal. eauto.
+    eapply (S_star2 EvtTau); eauto. econstructor.
+    eapply H. eauto.
+    econstructor; try eapply X. eauto. eauto.
+Qed.
+
+Lemma coproduces_reduction_closed S `{StateType S} (σ σ':S) L
+: coproduces σ L -> star2 step σ nil σ'  -> coproduces σ' L.
+Proof.
+  intros. general induction H1; eauto using coproduces. eauto.
+  destruct yl, y; simpl in *; try congruence.
+  eapply IHstar2; eauto.
+  eapply coproduces_reduction_closed_step; eauto.
+Qed.
+
+Lemma bisim_coproduces {S} `{StateType S} {S'} `{StateType S'} (sigma:S) (σ':S')
+  : bisim sigma σ' -> forall L, coproduces sigma L -> coproduces σ' L.
+Proof.
+  revert sigma σ'. cofix COH; intros.
+  inv H2.
+  - assert (bisim' σ'0 σ').
+    eapply bisim'_reduction_closed. eapply (bisim_bisim' H1).
+    eauto. econstructor.
+    exploit (bisim'_activated H4 H7). dcr.
+    edestruct H10. eauto. dcr.
+    econstructor; try eapply H8. eauto. eapply H11.
+    eapply COH; eauto.
+    eapply bisim'_bisim. eapply (bisim'_reduction_closed H7); eauto.
+    econstructor.
+  - econstructor. eapply (bisim_sound_diverges H1); eauto.
+  - exploit (bisim'_terminate H4 H5 (bisim_bisim' H1)).
+    dcr.
+    econstructor; eauto.
+Qed.
 
 
 
